\section{Power Series}
We look at series in the form 
\[
    \sum_{n=0}^{\infty} a_nz^n,\quad z\in \mathbb{C}, a_n\in \mathbb{C}.
\]
Or, for $ z_0 $ fixed, we look at 
\[
    \sum_{n=0}^{\infty} a_n(z-z_0)^n.
\]
\subsection{Radius of convergence}
\begin{lemma}
    If $ \sum_{n=0}^{\infty} a_n z_1^n$ converges, and $ |z|<|z_1| $, then $ \sum_{n=0}^{\infty} a_n z^n $ converges absolutely.
\end{lemma}
\begin{proof}
    Since $ \sum_{n=0}^{\infty} a_n z_1^n$ converges, $a_nz_1^n\to 0$. Thus $ \{a_nz_1^n\} $ is bounded by $K>0$. Now 
    \[
        \left| a_nz^n \right| \le K \left| \frac{z}{z_1} \right| ^n.
    \]
    Since the sum of RHS converges, the lemma follows by comparison.
\end{proof}
Using this lemma we will show that every power series has a radius of convergence.
\begin{theorem}\label{thm:4.2}
    A power series either
    \begin{enumerate}
        \item converges absolutely for all $z$, or
        \item converges absolutely for all $z$ inside a circle $ |z|=R, R> 0 $, and diverges for all $ |z|>R $, or 
        \item converges for $R=0$ only.
    \end{enumerate}
\end{theorem}
\begin{definition}[Radius of convergence]
    The circle $ |z|=R $ is called the \textbf{circle of convergence} and $R$ is the \textbf{radius of convergence}.
\end{definition}
\begin{proof}
    Let $ S = \{x\in \mathbb{R}: x\ge 0 \land \sum a_n x^n \text{ converges}\} $. Clearly $0\in S$. If $ x_1\in S, [0,1]\in S $. If $ S=[0,\infty) $ then we have case 1. If not, $ \exists R = \sup S \ge 0 $ finite.

    If $ R>0 $, We will prove that if $ |z_1|<R $ then $ \sum a_nz_1^n $ converges absolutely. Choose $ R_0 $ such that $ |z_1|<R_0<R $. Then $ R_0\in S $ by definition of sup, and the series converges for $ z=R_0 $. By lemma, $ \sum |a_n z^n| $ converges.

    Finally we show that if $ |z_2|>R\ge 0 $, then the series does not converge. Take $ R_0 $ such that $ R<R_0<|z_2| $. If $ \sum a_nz_2^n $ converges, then $ \sum a_n R_0^n $ converges, contradicting with the choice of $R_0$.
\end{proof}

The following lemma is useful for finding $R$: 
\begin{lemma}\label{lma:4.3}
    If $ |a_{n+1}/a_n|\to \ell $, then $ R = 1/\ell $.
\end{lemma}
\begin{proof}
    By ratio test, we have absolute convergence if 
    \[
        \lim_{n \to \infty} \left| \frac{a_{n+1}}{a_n}\frac{z^{n+1}}{z^n} \right| <1, 
    \]
    so if $ |z|<\frac{1}{\ell} $, we have absolute convergence. If $ |z|>\frac{1}{\ell} $, then the series diverges.
\end{proof}
\begin{remark}
    One can also use root test to get that $ |a_n|^{1/n}\to \ell $, then $ R = 1/\ell $.
\end{remark}
\begin{example}
    \begin{enumerate}
        \item $\displaystyle \sum_{n=0}^{\infty}\frac{z^n}{n!}$. Note that 
        \[
            \left| \frac{a_{n+1}}{a_n} \right|  = \frac{1}{n+1}\to 0=\ell,
        \]
        so $ R=\infty $.
        \item $\displaystyle \sum_{n=0}^{\infty}z^n$. Immediately $ R=1 $. Note that on the circle we have divergence.
        \item $\displaystyle \sum_{n=0}^{\infty}n!z^n$. Clearly $ R=0 $.
        \item $\displaystyle \sum_{n=1}^{\infty}\frac{z^n}{n}$. $ R=1 $. But it diverges for $z=1$. If $ |z|=1,z\neq 1 $, it converges by Abel's test (see example sheet 1). Alternatively, consider 
        \[
            \sum_{n=1}^{\infty}\frac{z^n}{n}(1-z) \Longrightarrow \begin{aligned}
                s_N &= \sum_{n=1}^{N}\left( \frac{z^n-z^{n+1}}{n} \right) = \sum_{n=1}^{N}\frac{z^n}{n}-\sum_{n=2}^{N+1}\frac{z^{n}}{n-1}\\ 
                &= z-\frac{z^{N+1}}{N}+ \sum_{n=2}^{N+1}\frac{-z^n}{n(n-1)}.
            \end{aligned}
        \]
        If $ |z|=1 $, then $ \frac{z^{N+1}}{N}\to 0 $ and $ \sum_{n=2}^{\infty}\frac{1}{n(n-1)} $, so $s_N$ converges.
        \item $\displaystyle \sum_{n=1}^{\infty} \frac{z^n}{n^2}$. $ R=1 $ and it converges for all $z$ with $|z|=1$.
        \item $\displaystyle \sum_{n=0}^{\infty} nz^n$. $ R=1 $ but it diverges for all $ |z|=1 $.  
    \end{enumerate}
\end{example}
\begin{remark}
    \textit{No} claim is made \textit{on} the circle of convergence. Within the radius of convergence, power series will behave as if they were polynomials.
\end{remark}

\subsection{Differentiation}
\begin{theorem}\label{thm:4.4}
    Suppose the series
    \[
        f(z) = \sum_{n=0}^{\infty}a_n z^n
    \]
    has radius of convergence $R$. Then $f$ is differentiable at all points $ |z|<R $ with derivative 
    \[
        f'(z) = \sum_{n=1}^\infty na_n z^{n-1}.
    \]
\end{theorem}
\begin{proof}
    We need 2 lemmas:
    \begin{lemma}\label{lma:4.5}
        If $ \sum_0^\infty a_nz^n $ has radius of convergence $R$, then so do $ \sum_{1}^{\infty}na_n z^{n-1} $ and $ \sum_{2}^\infty n(n-1)a_n z^{n-2} $.
    \end{lemma}
    \begin{lemma}\label{lma:4.6}
        \begin{enumerate}
            \item For all $2\le r\le n$, $\displaystyle \binom{n}{r}\le n(n-1) \binom{n-2}{r-2}$.
            \item $ \left| (z+h)^n-z^n-nhz^{n-1} \right| \le n(n-1)(|z|+|h|)^{n-2}|h|^2,\ \forall z,h\in \mathbb{C} $. 
        \end{enumerate}
    \end{lemma}

    By lemma 4.5 we may define 
    \[
        f'(z) := \sum_{n=1}^{\infty} na_n z^{n-1},\quad |z|<R.
    \]
    We are required to prove that 
    \[
        \lim_{h \to 0} I = \lim_{h \to 0} \frac{f(z+h)-f(z)-hf'(z)}{h}=0.
    \]
    Note that (by lemma 4.6),
    \begin{IEEEeqnarray*}{rCl}
        I &=& \frac{1}{h}\sum_{n=0}^{\infty} a_n((z+h)^n-z^n-hnz^{n-1})\\ 
        \Longrightarrow  |I| &=& \frac{1}{|h|}\left| \lim_{N \to \infty} \sum_{n=0}^{N} a_n((z+h)^n-z^n-hnz^{n-1})\right|\\ 
        &=& \frac{1}{|h|}\lim_{N \to \infty}\left|  \sum_{n=0}^{N} a_n((z+h)^n-z^n-hnz^{n-1})\right|\\ 
        &\le& \frac{1}{|h|}\sum_{n=0}^{\infty} |a_n||(z+h)^n-z^n-hnz^{n-1}|\\ 
        &\le& \frac{1}{|h|}\sum_{n=2}^{\infty}|a_n|\cdot n(n-1)(|z|+|h|)^{n-2}|h|^2\\ 
        &=& |h|\sum_{n=2}^{\infty} |a_n| \cdot n(n-1)(|z|+|h|)^{n-2}
    \end{IEEEeqnarray*}
    By lemma 4.5, for $|h|$ small enough, 
    \[
        \sum_{n=2}^{\infty} |a_n| \cdot n(n-1)(|z|+|h|)^{n-2}
    \]
    converges to $A(h)$, but $A(h)\le A(r)$ for $r$ such that $|h|<r$ and $ |z|+r<R $. Hence 
    \[
        0\le |I|\le |h|A(h) \le |h|A(r)\to 0 \quad \text{as}\quad h\to 0,
    \]
    as required.
\end{proof}
\begin{proof}[Proof of lemma 4.5]
    The lemma holds trivially for $z=0$.
    Take $z,R_0$ such that $ 0<|z|<R_0<R $. Since $ a_nR_0^n\to 0 $, $ \exists K $ such that $ |a_n R_0^n|\le K, \forall n\ge 0 $. Thus 
    \[
        \left| a_n n z^{n-1} \right| = \frac{n}{|z|} \left| a_n R_0^n \right| \left| \frac{z}{R_0} \right|^n \le \frac{Kn}{|z|}\left| \frac{z}{R_0} \right|^n.
    \]
    But the series $\sum \frac{n}{|z|}| \frac{z}{R_0} |^n$ converges by the ratio test (check it), so $ \sum a_n n z^{n-1} $ converges absolutely by comparison, thus converges.

    If $ |z|>R $, then $ |a_nz^n| $ is \textit{unbounded} (check \href{https://math.stackexchange.com/questions/799481/absolute-sequence-unbounded-within-radius-of-convergence}{this}), and so is $ n|a_nz^n| $, so $ \sum na_n z^{n-1} $ diverges. The same proof applies to $\sum_{2}^\infty n(n-1)a_n z^{n-2}$.
\end{proof}
\begin{proof}[Proof of lemma 4.6]
    Part 1 follows by direct check. For part 2, note that
    \[
        (z+h)^n-z^n-nhz^{n-1} = \sum_{r=2}^{n}\binom{n}{r} z^{n-r}h^r.
    \] 
    Thus 
    \begin{align*}
        \left| (z+h)^n-z^n-nhz^{n-1} \right| &\le \sum_{r=2}^{n}\binom{n}{r} |z|^{n-r}|h|^r \\ 
        &\le |h|^2 n(n-1) \sum_{r=2}^{n}\binom{n-2}{r-2}|z|^{n-r}|h|^{r-2}\\
        &= n(n-1)(|z|+|h|)^{n-2}|h|^2. \qedhere
    \end{align*}
\end{proof}

\subsection{The standard functions}
\subsubsection*{Exponentials and logarithms}
We have already seen that 
\[
    \sum_{n=0}^{\infty} \frac{z^n}{n!}
\]
has $ R=\infty $.
\begin{definition}
    The \textbf{exponential function} is defined by $ e:\mathbb{C}\to\mathbb{C} $, where
    \[
        e(z) = \sum_{n=0}^{\infty} \frac{z^n}{n!}.
    \]
\end{definition}
Straight from theorem \ref{thm:4.4}, $ e $ is differentiable and $ e'(z)=e(z) $.

\begin{sprop}
    If $ F:\mathbb{C}\to\mathbb{C} $ has $ F'(z)=0, \forall z\in \mathbb{C} $, then $F$ is constant.
\end{sprop}
\begin{proof}
    Consider $g(t)=F(tz)=u(t)+iv(t)$. By chain rule,
    \[
        g'(t)=F'(tz)z=0=\footnote{Check}u'(t)+iv'(t) \Longrightarrow u'=v'=0.
    \]
    Hence $u,v$ are constant by corollary \ref{col:3.5}, thus $F$ is constant.
\end{proof}

Now let $a,b\in \mathbb{C}$ and consider 
\[
    F(z) = e(a+b-z)e(z) \Longrightarrow F'(z) = 0.
\]
So $F$ is constant and $e(a+b-z)e(z)=e(a+b).$ Set $z=b$ gives 
\[
    \boxed{e(a)e(b)=e(a+b)} 
\]

Now we restrict $ e:\mathbb{R} \to \mathbb{R} $.

\begin{theorem}[Properties of the exponential]\label{thm:4.7}\
    \begin{enumerate}
        \item $ e:\mathbb{R}\to\mathbb{R} $ is differentiable on $\mathbb{R}$ with $ e'(x)=e(x) $.
        \item $ e(x+y)=e(x)e(y) $.
        \item $ e(x)>0 $.
        \item $ e $ is strictly increasing.
        \item $ e(x)\to \infty $ as $ x\to \infty $, $ e(x)\to 0 $ as $ x\to -\infty  $.
        \item $ e:\mathbb{R} \to (0,\infty) $ is a bijection.
    \end{enumerate}
\end{theorem}
\begin{proof}
    1 and 2 are done by previous. 3: clearly $ e(x)>0, \forall x\ge 0 $ and $ e(0)=1>0 $. By property 2, $ e(x)>0, \forall x<0 $, and hence $ e(x)>0, \forall x\in \mathbb{R} $. 4: $ e'(x)=e(x)>0 $, so $e$ is strictly increasing. 5: from the definition of $e(x)$, $ e(x)>1+x $. As $ x\to \infty, 1+x\to \infty   $ and thus $ e(x)\to \infty $. Also since $ e(-x)=1/e(x) $ by property 2, $ e(x)\to 0, x\to -\infty  $. 6: injectivity follows by strict increasing property. Take $ y\in (0,\infty ) $. By property 5, $ \exists a,b \in \mathbb{R} $ such that $ e(a)<y<e(b) $. By IVT, $ \exists x\in \mathbb{R}, e(x)=y $, so $e$ is surjective, hence bijective.
\end{proof}
\begin{remark}
    $ e:(\mathbb{R} ,+)\to ((0,\infty ),\times ) $ is an isomorphism.
\end{remark}

\begin{definition}
    The \textbf{logarithm} is defined by the inverse of exponential: $ l:(0,\infty )\to \mathbb{R}  $.
\end{definition}
\begin{theorem}[Properties of logarithm]\label{thm:4.8}\
    \begin{enumerate}
        \item $ l:(0,\infty )t\to \mathbb{R}  $ is a bijection and $ l(e(x))=x, \forall x\in \mathbb{R} $, $ e(l(t))=t,\forall t\in (0,\infty ) $.
        \item $l$ is differentiable with derivative $ e'(t)=1/t $.
        \item $ l(xy)=l(x)+l(y),\forall x,y\in (0,\infty ) $.
    \end{enumerate}
\end{theorem}
\begin{proof}
    Exercise.
\end{proof}

\subsubsection*{Power functions}

\begin{definition}
    Given $ \alpha\in \mathbb{R}, x>0 $, define the \textbf{power function} $ r_\alpha:\mathbb{R} \to \mathbb{R} $ as 
    \[
        r_\alpha(x) := e(\alpha l(x)).
    \]
\end{definition}
\begin{theorem}[Properties of powers]\label{thm:4.9}
    Suppose $ x,y>0,\alpha,\beta\in \mathbb{R} $. Then 
    \begin{enumerate}
        \item $ r_\alpha(xy)=r_\alpha(x)r_\alpha(y) $.
        \item $ r_{\alpha+\beta}(x)r_\alpha(x)r_\beta(x) $.
        \item $ r_\alpha(r_\beta(x))=r_{\alpha\beta}(x) $.
        \item $ r_1(x)=x,r_0(x)=1 $.
    \end{enumerate}
\end{theorem}
\begin{proof}
    Exercise.
\end{proof}

In particular, $ r_n(x)=r_1(x)^n=x^n $, and $ r_{-1}(x)=1/x $, and thus $ r_{-n}(x)=1/x^n $. Similar process can be applied to $ r_q(x),q\in \mathbb{Q} $.

Now we do a ``Baptism Ceremony'':
\[
    \begin{cases}
    \exp (x):=e(x) &x\in \mathbb{R} \\
    \log x :=l(x) &x\in (0,\infty )\\
    x^{\alpha}:= r_\alpha(x) & x\in (0,\infty ),\alpha\in \mathbb{R}
    \end{cases} 
\]
One can deduce, for example, that 
\[
    \exp (x)=\exp (x \log \exp (1) ) = r_x(\exp (1)) = (\exp (1))^x.
\]
Thus $\exp(x)$ is also a power and we can define 
\[
    \boxed{e:= \exp (1) = \sum_{n=0}^{\infty}\frac{1}{n!}}
\]
We may denote 
\[
    e^x:= \exp (x).
\]
\begin{sprop}
    $ (x^\alpha)'=\alpha x^{\alpha-1} $.
\end{sprop}
\begin{proof}
    $ (x^\alpha)'=(e^{\alpha \log x})'=e^{\alpha \log x}\cdot \alpha/x = \alpha x^{\alpha-1} $.
\end{proof}
\begin{note}
    If we let $ f(x)=a^x,a>0 $, then $ f'(x)=a^x\log a $.
\end{note}

\begin{sprop}[Exponentials beat polynomials]
    $\displaystyle \lim_{x \to \infty} \frac{e^x}{x^k}\to \infty, \forall k\in \mathbb{Z}$. 
\end{sprop}
\begin{proof}
    Wlog suppose $x>0$. Let $n>k$ such that 
    \[
        e^x = \sum_{j=0}^{\infty} \frac{x^j}{j!}>\frac{x^n}{n!}.
    \]
    Hence 
    \[
        \frac{e^x}{x^k}>\frac{x^{n-k}}{n!}\to \infty,\quad \text{as }x\to \infty .\qedhere
    \]
\end{proof}

\subsection{Trignometric functions}
\begin{definition}
    Define $ \sin ,\cos : \mathbb{C} \to \mathbb{C} $ as 
    \begin{align*}
        \cos z &= 1-\frac{z^2}{2!}+\frac{z^4}{4!}-\cdots = \sum_{k=0}^{\infty} \frac{(-1)^k z^{2k}}{(2k)!},\\ 
        \sin z &= z-\frac{z^3}{3!}+\frac{z^5}{5!}-\cdots = \sum_{k=0}^{\infty}\frac{(-1)^k z^{2k+1}}{(2k+1)!}.
    \end{align*}
\end{definition}

\begin{sprop}
    \begin{enumerate}
        \item     $ \sin z,\cos z $ has infinite radius of convergence and are differentiable with $ \sin(z)'= \cos(z) $ and $ \cos(z)'=-\sin (z) $.
        \item $ e^{iz}=\cos z+i \sin z $ and $ e^{-iz}=\cos z-i \sin z $.
        \item $\displaystyle \cos z=\frac{1}{2}\left( e^{iz}+e^{-iz} \right)$, and $\displaystyle \sin z = \frac{1}{2i}\left( e^{iz}-e^{-iz} \right)$. 
        \item $\forall z\in \mathbb{C},\ \sin ^2 z+ \cos ^2 z=1 $.
        \item All trignometric identities hold.
        \item $ \mathbb{R}\ni y\to \infty,\ \cos(iy)\to \infty $.
        \item If $ x\in \mathbb{R},\ \sin x, \cos x\in \mathbb{R} $.
        \item $ \forall x\in \mathbb{R},\ |\sin x|,|\cos x|\le 1 $.
    \end{enumerate}
\end{sprop}

\begin{proposition}\label{prop:4.10}
    $ \exists \omega\in \mathbb{R},\ \sqrt{2}<\omega/2<\sqrt{3} $, such that 
    \[
        \cos \frac{\omega}{2}=0.
    \]
\end{proposition}
\begin{proof}
    It is clear that if $0<x<2$, $ \sin x>0 $. So for $0<x<2$, $ (\cos x)'=- \sin x<0 $, so $\cos x$ is strictly decreasing on $ (0,2) $. Claim that $ \cos \sqrt{2}>0, \cos \sqrt{3}<0 $, so by IVT the existence of $ \omega $ follows. Indeed, 
    \begin{align*}
        \cos \sqrt{2}&= \left( \frac{(\sqrt{2})^4}{4!}- \frac{(\sqrt{2})^6}{6!}\right)+\cdots>0\\ 
        \cos \sqrt{3}&= -\frac{1}{8}- \left( \frac{(\sqrt{2})^6}{6!}-\frac{(\sqrt{2})^8}{8!} \right)- \cdots <0.\qedhere
    \end{align*}
\end{proof}

\begin{definition}
    Define $ \pi=\omega $.
\end{definition}

\begin{theorem}\label{thm:4.12}
    \begin{enumerate}
        \item $ \sin (z+\pi/2)=\cos z $, $ \cos (z+\pi/2)=-\sin z $.
        \item $ \sin (z+\pi)=-\sin z,\ \cos (z+\pi)=-\cos z $.
        \item $ \sin (z+2\pi)=\sin z,\ \cos (z+2\pi)=\cos z $.
    \end{enumerate}
\end{theorem}

This implies 
\[
    e^{iz+2\pi i}=\cos (z+2\pi)+i \sin (z+2\pi)= e^{iz},
\]
so $e^z$ is periodic with period $ 2\pi i $.

\begin{remark}[Relation with geometry]
    Given 2 vectors $ \mathbf{x},\mathbf{y}\in \mathbb{R}^{2} $, we have by Cauchy-Schwarz that $ |\mathbf{x} \cdot \mathbf{y}|<|bfx|\mathbf{y}| $. Thus for $ \mathbf{x},\mathbf{y}\neq \mathbf{0} $, we have 
    \[
        -1\le \frac{\mathbf{x}\cdot\mathbf{y}}{|\mathbf{x}||\mathbf{y}|}\le 1.
    \]
    So we can define the \textbf{angle} between $\mathbf{x},\mathbf{y}$ as $ \theta\in [0,2\pi] $ such that 
    \[
        \cos \theta=\frac{\mathbf{x}\cdot\mathbf{y}}{|\mathbf{x}||\mathbf{y}|}.
    \]
\end{remark}

\subsection{Hyperbolic functions}
\begin{definition}
    Define $ \sinh ,\cosh : \mathbb{C} \to \mathbb{C} $ as 
    \[
        \sinh z = \frac{e^z-e^{-z}}{2},\quad \cosh z = \frac{e^z+e^{-z}}{2}.
    \]
\end{definition}
One can easily check that 
\begin{sprop}
    \begin{enumerate}
        \item $ \cosh z = \cos iz,\ \sinh z = -i \sin iz. $
        \item $ (\cosh z)'=\sinh z,\ (\sinh z)'=\cosh z .$
        \item $ \cosh^2 z-\sinh^2 z=1 $, etc.
    \end{enumerate}
\end{sprop}

The rest of the trignometric functions are defined in the usual way.